Before continuing let us prove some useful facts about Boolean algebras.
\begin{theorem*}
If $\langle B, \meet, \join, ', 0 , 1\rangle$ is a Boolean algebra then $x \join 0 = x$ and $x \meet 1 = x$ for all $x\in B$.
\end{theorem*}

\begin{proof}
Assume  $\langle B, \meet, \join, ', 0 , 1\rangle$ is a Boolean algebra and take any $x \in B$.
Then
\begin{align*}
  x &= x \join (x \meet 0)           & \text{Lattice absorbtion}\\
    &= x \join 0                     & \text{Boolean algebra}
\end{align*}
Dually,
\begin{align*}
  x &= x \meet (x \join 1)           & \text{Lattice absorbtion}\\
    &= x \meet 1                     & \text{Boolean algebra}
\end{align*}
\end{proof}

\begin{theorem*}
If $\langle B, \meet, \join, ', 0 , 1\rangle$ is a Boolean algebra then $(x \join y)' = (x' \meet y')$ and $(x \meet y)' = (x' \join y')$ for all $x, y\in B$.
\end{theorem*}
\begin{proof}
Assume $\langle B, \meet, \join, ', 0 , 1\rangle$ is a Boolean algebra.
Then
\begin{align*}
(x\join y) \meet (x' \meet y') &= ((x\join y) \meet x') \meet y' \\
                               &= (x' \meet  (x\join y)) \meet y' \\
                               &= ((x' \meet x) \join (x' \meet y)) \meet y' \\
                               &= (0 \join (x' \meet y)) \meet y' \\
                               &= (x' \meet y) \meet y' \\
                               &= x' \meet (y \meet y') \\
                               &= x' \meet 0 \\
                               &= 0 
\end{align*}
Furthermore,
\begin{align*}
(x\join y) \join (x' \meet y') &= x\join (y \join (x' \meet y')) \\
                               &= x\join ((y \join x') \meet (y \join y')) \\
                               &= x\join ((y \join x') \meet 1) \\
                               &= x\join (y \join x') \\
                               &= x\join (x' \join y) \\
                               &= (x\join x') \join y \\
                               &= 1 \join y \\
                               &= 1
\end{align*}
Therefore $x' \meet y'$ is a complement of $x\join y$ and since there is at most one complement for an element of a boolean algebra, $x' \meet y' = (x\join y)'$. A similar proof shows that $x' \join y' = (x\meet y)'$
\end{proof}

\begin{theorem*}
If $\langle B, \meet, \join, ', 0 , 1\rangle$ is a Boolean algebra then $(x')' = x$.
\end{theorem*}

\begin{proof}
\begin{align*}
  (x')' &= 1 \meet (x')' \\
        &= (x \join x') \meet (x')'  \\
        &= (x')' \meet (x \join x') \\
        &= ((x')' \meet x) \join ((x')' \meet x') \\
        &= ((x')' \meet x) \join 0 \\
        &= (x')' \meet x
\end{align*}
So $(x')' \leq x$.
Next,
\begin{align*}
  x &= x \meet 1 \\
    &= x \meet (x' \join (x')') \\
    &= (x \meet x') \join (x \meet (x')') \\
    &= 0 \join (x \meet (x')') \\
    &= x \meet (x')' \\
\end{align*}
So $x \leq (x')'$.
Therefore $x = (x')'$ by anti-symmetry because $(x')' \leq x$ and $x \leq (x')'$.
\end{proof}

\begin{theorem*}
If $\langle B, \meet, \join, ', 0 , 1\rangle$ is a Boolean algebra and $a, b \in B$, define $a\to b$ to be $a'\join b$.
Then $\langle B, \meet, \join, \to, 0, 1\rangle$ is a Heyting algebra.
\end{theorem*}

\begin{proof}
Assume $\langle B, \meet, \join, ', 0 , 1\rangle$ is a Boolean algebra and define $a\to b$ as $a'\join b$ for all $a, b \in B$.
Then for any $x, y, z \in B$
\begin{enumerate}[(H1)]
  \item Follows from B1.
  \item Follows from B2.
  \item $x\to x = x'\join x = 1$
  \item 
    \begin{align*}
      (x\to y) \meet y &= (x' \join y) \meet y & \text{$x\to y = x' \join y$} \\
                       &= y \meet (x' \join y) & \text{Lattice commutativity} \\
                       &= y \meet (y \join x') & \text{Lattice commutativity}\\
                       &= y                    & \text{Lattice absorbtion}
    \end{align*}
    Furthermore
    \begin{align*}
      x \meet (x\to y) &= x \meet (x' \join y) \\
                       &= (x \meet x') \join (x \meet y) \\
                       &= 0 \join (x \meet y) \\
                       &= x \meet y \\
    \end{align*}
  \item 
    \begin{align*}
      x \to (y \meet z) &= x' \join (y \meet z) \\ 
                        &= (x' \join y) \meet (x' \join z) \\
                        &= (x \to y) \meet (x \to z)
    \end{align*}
    And
    \begin{align*}
      (x \join y) \to z &= ((x \join y)' \join z) \\
                        &= ((x' \meet y') \join z) \\
                        &= (x'\join z) \meet (y'\join z) \\
                        &= (x\to z) \meet (y\to z)
    \end{align*}
\end{enumerate}
Therefore the $\langle B, \meet, \join, \to, 0, 1\rangle$ satisfies H1-5 and is a Heyting algebra.
\end{proof}

